Reorganize files and directories

lib/misc.v
@@ -1,28 +1,7 @@
-From stdpp Require Export gmap.
+From iris.algebra Require Import local_updates gset.
 
-From iris.heap_lang Require Export notation.
-
-
-Definition oloc_to_val (ol: option loc) : val := 
-  match ol with
-  | None => NONEV
-  | Some l => SOMEV #l
-  end.
 
 Local Open Scope Z.
-Definition node_rep : Type := Z * option loc * val.
-Definition node_key (n: node_rep) : Z := n.1.1.
-Definition node_next (n: node_rep) : option loc := n.1.2.
-Definition node_lock (n: node_rep) : val := n.2.
-
-Definition node_lt (x y: node_rep) : Prop := 
-  node_key x < node_key y.
-
-Definition rep_to_node (n: node_rep) : val :=
-  (#(node_key n), oloc_to_val (node_next n), (node_lock n)).
-
-Definition key_equiv (S: gset node_rep) (Skeys: gset Z) :=
-  Permutation (elements Skeys) (map node_key (elements S)).
 
 Fixpoint Zset_inclusive_range (z: Z) (gap : nat) : gset Z :=
   match gap with
@@ -35,3 +14,177 @@ Definition Zset_exclusive_range (z: Z) (gap: nat) : gset Z :=
 
 Definition Zlt_range (z1 z2: Z) : gset Z := 
   Zset_exclusive_range z1 (Z.to_nat (z2 - z1)).
+
+
+Lemma in_inv {A: Type} :
+  forall (l: list A) (a b: A) , In b (a :: l) ↔ b = a ∨ In b l.
+Proof.
+  intros l a b. split; intros H.
+  + destruct l as [|c l]; inversion H; auto.
+  + inversion H.
+    - by left.
+    - by right.
+Qed.
+
+Lemma in_inv_rev {A: Type} :
+  forall (l: list A) (a b: A) , In b (l ++ [a]) ↔ In b l ∨ b = a.
+Proof.
+  intros l a b. split; intros H.
+  + induction l as [|c l] using rev_ind.
+    - inversion H; auto; by exfalso.
+    - apply in_app_or in H. inversion H as [?|H'].
+      * auto.
+      * inversion H'; auto; by exfalso.
+  + inversion H.
+    - apply in_or_app. by left.
+    - apply in_or_app. right. by left.
+Qed.
+
+Lemma no_dup_elem_unique {A: Type} (L1 L2 L1' L2': list A) elem elem1 elem2 :
+  NoDup (L1 ++ elem1 :: elem :: L2) →
+  L1 ++ elem1 :: elem :: L2 = L1' ++ elem2 :: elem :: L2' →
+  elem1 = elem2.
+Proof.
+  rewrite NoDup_ListNoDup.
+  revert L2 L1' L2'.
+  induction L1 => //=.
+  - intros L2 L1' L2' Hno_dup Heq.
+    destruct L1' as [| a L1'].
+    * rewrite //= in Heq; congruence. 
+    * destruct L1' as [| b L1'].
+      ** rewrite //= in Heq. assert (L2 = elem :: L2') by congruence.
+        subst. exfalso.
+        rewrite ?NoDup_cons_iff in Hno_dup *.
+        destruct Hno_dup as [Hpred Hno_dup].
+        destruct Hno_dup as [Hnp Hno_dup].
+        destruct Hno_dup as [Hnp' Hno_dup].
+        apply Hnp. by left.
+      ** rewrite //= in Heq. assert (L2 = L1' ++ (elem2 :: elem :: L2')) by congruence.
+        subst. 
+        rewrite ?NoDup_cons_iff in Hno_dup *.
+        destruct Hno_dup as [Hpred Hno_dup].
+        destruct Hno_dup as [Hnp Hno_dup].
+        exfalso. apply Hnp.
+        apply in_or_app. right. econstructor; econstructor. auto.
+  - intros L2 L1' L2' Hnd.
+    destruct L1' as [| a' L1'].
+    { rewrite //=.
+      rewrite -NoDup_ListNoDup NoDup_cons in Hnd; destruct Hnd as [Ha Hnd].
+      rewrite NoDup_app in Hnd; destruct Hnd as [Hl1 Hnd]; destruct Hnd as [Hx Hnd].
+      intros Heq.
+      cut (elem = elem1 ∨ In elem L1).
+      { intros [Heqpred1|Hin].
+        * exfalso.  subst.
+          inversion Hnd as [|? ? Hpred Hnd']; subst.
+          eapply Hpred. by left.
+        * exfalso.  eapply Hx. 
+          ** apply elem_of_list_In; eauto.
+          ** right. by left.
+      }
+      destruct L1.
+      * rewrite //= in Heq. inversion Heq; subst; auto.
+      * right. inversion Heq; subst. by left.
+    }
+    inversion 1; subst. eapply IHL1; eauto.
+    inversion Hnd; eauto.
+Qed.
+
+Lemma no_dup_inj_in_map {T1 T2: Type} (f: T1 → T2) (l: list T1) :
+  (∀ x y, In x l → In y l → f x = f y → x = y) →
+  NoDup l → NoDup (map f l).
+Proof.
+  intros Hinj.
+  induction 1 as [|a l Hnin Hnd IH]; first constructor.
+  rewrite //=. constructor.
+  + intros Hin_map.
+    rewrite elem_of_list_In in_map_iff in Hin_map.
+    destruct Hin_map as [x Hin].
+    destruct Hin as [Heq Hin].
+    apply Hinj in Heq; subst.
+    - destruct Hnin. rewrite elem_of_list_In //.
+    - by right.
+    - by left.
+  + eapply IH. intros. eapply Hinj; last done. 
+    all: by right.
+Qed.
+
+Lemma Zset_inclusive_range_spec z gap:
+  ∀ z', z' ∈ (Zset_inclusive_range z gap) ↔ (z <= z' <= z + gap).
+Proof.
+  induction gap.
+  + rewrite //= => z'. split.
+    - intros ?%elem_of_singleton. subst. lia.
+    - intros (?&?); assert (z = z') as -> by lia. rewrite elem_of_singleton //.
+  + rewrite /Zset_inclusive_range -/Zset_inclusive_range => z'. split.
+    - intros [Hspz%elem_of_singleton|Hrec]%elem_of_union.
+      * lia.
+      * destruct (IHgap z') as (Himp&?). specialize (Himp Hrec). lia.
+    - intros (?&Hle).
+      apply Zle_lt_or_eq in Hle as [Hlt|?].
+      * apply elem_of_union_r. eapply IHgap. lia.
+      * apply elem_of_union_l. rewrite elem_of_singleton //.
+Qed.
+
+Lemma Zset_exclusive_range_spec z gap:
+  ∀ z', z' ∈ (Zset_exclusive_range z gap) ↔ (z < z' < z + gap).
+Proof.
+  intros z'. split.
+  - rewrite /Zset_exclusive_range.
+    intros (Hincl&Hneq)%elem_of_difference.
+    apply Zset_inclusive_range_spec in Hincl.
+    assert (z' ≠ z ∧ z' ≠ z + gap) by set_solver.
+    lia.
+  - rewrite /Zset_exclusive_range. 
+    intros Hrange.
+    apply elem_of_difference; split.
+    * apply Zset_inclusive_range_spec; lia.
+    * assert (z' ≠ z ∧ z' ≠ z + gap) by lia.
+      set_solver.
+Qed.
+
+Lemma Zlt_range_spec z1 z2:
+  ∀ z', z' ∈ (Zlt_range z1 z2) ↔ (z1 < z' < z2).
+Proof.
+  intros z'.
+  rewrite /Zlt_range Zset_exclusive_range_spec; lia.
+Qed.
+
+Lemma Zlt_range_split z1 z2 z:
+  z1 < z < z2 → Zlt_range z1 z2 = Zlt_range z1 z ∪ Zlt_range z z2 ∪ {[ z ]}.
+Proof.
+  intros Hrange.
+  rewrite -leibniz_equiv_iff.
+  intros x. split.
+  + rewrite Zlt_range_spec. intros.
+    destruct (Ztrichotomy_inf x z) as [[Hlt|Heq]|Hgt].
+    - do 2 apply elem_of_union_l. rewrite Zlt_range_spec. lia.
+    - apply elem_of_union_r. rewrite elem_of_singleton //.
+    - apply elem_of_union_l, elem_of_union_r. rewrite Zlt_range_spec. lia.
+  + rewrite Zlt_range_spec. 
+    intros [[Hin|Hin]%elem_of_union|Hin]%elem_of_union. 
+    - rewrite Zlt_range_spec in Hin *; lia.
+    - rewrite Zlt_range_spec in Hin *; lia.
+    - apply elem_of_singleton in Hin; lia.
+Qed.
+
+Lemma Zlt_range_split_op z1 z2 z:
+  z1 < z < z2 → GSet (Zlt_range z1 z2) = 
+    GSet (Zlt_range z1 z) ⋅ GSet (Zlt_range z z2) ⋅ GSet ({[ z ]}).
+Proof.
+  intros Hrange. rewrite (Zlt_range_split z1 z2 z) //.
+  rewrite ?gset_disj_union; auto.
+  + intros z' [Hin%Zlt_range_spec|Hin%Zlt_range_spec]%elem_of_union.
+    - rewrite elem_of_singleton //; lia.
+    - rewrite elem_of_singleton //; lia.
+  + intros z'. rewrite ?Zlt_range_spec. lia.
+Qed.
+
+Section gset_extra.
+  Context `{Countable K}.
+  Implicit Types X Y Z : gset K.
+  Lemma gset_local_update_union X Y W : (X,Y) ~l~> (X ∪ W,Y ∪ W).
+  Proof.
+    rewrite local_update_unital_discrete=> Z' _ /leibniz_equiv_iff->.
+    split. done. rewrite gset_op. set_solver.
+  Qed.
+End gset_extra.
