lazy_list/node_lt.v
@@ -1,0 +1,245 @@
+From Coq Require Import Lia.
+From Coq Require Import Sorting.Sorted.
+
+From iris.heap_lang Require Import notation.
+
+From SkipList.lazy_list Require Import code node_rep.
+
+
+Local Open Scope Z.
+
+Module NodeLt (Params: LAZY_LIST_PARAMS).
+  Import Params.
+  Module Code := LazyList Params.
+  Export Code.
+
+
+  Definition node_lt (x y: node_rep) : Prop := 
+    node_key x < node_key y.
+
+
+  Lemma node_lt_transitive :
+    forall x y z, node_lt x y → node_lt y z → node_lt x z.
+  Proof.
+    intros x y z. unfold node_lt.
+    intros xy yz. lia.
+  Qed.
+
+  Lemma node_lt_le_incl : 
+    ∀ x y, node_lt x y → node_key x ≤ node_key y.
+  Proof.
+    intros x y Hlt.
+    unfold node_lt in Hlt. lia.
+  Qed.
+
+  Lemma node_rep_sorted_eq (l l': list node_rep) :
+    Sorted node_lt l →
+    Sorted node_lt l' →
+    Permutation l l' →
+    l = l'.
+  Proof.
+    revert l'.
+    induction l.
+    - intros l' ?? ?%Permutation.Permutation_nil. subst. auto.
+    - intros l' Hsorted Hsorted' Hperm.
+      destruct l' as [| a' l'].
+      { symmetry in Hperm. apply Permutation.Permutation_nil in Hperm. congruence. } 
+      destruct_decide (decide (a = a')) as Hcase.
+      { intros; subst.  f_equal.
+        eapply IHl.
+        { eapply Sorted_inv; eauto. }
+        { eapply Sorted_inv; eauto. }
+        apply Permutation.Permutation_cons_inv in Hperm; eauto.
+      }
+      
+      exfalso. cut (node_key a < node_key a' ∧ node_key a' < node_key a); first lia.
+      split.
+      * apply Sorted_StronglySorted in Hsorted; last eauto with *.
+        inversion Hsorted as [| ??? Hall]; subst.
+        assert (List.In a' (a :: l)) as [|]; subst.
+        { apply elem_of_list_In. rewrite Hperm. by left. }
+        ** congruence. 
+        ** eapply List.Forall_forall in Hall; eauto.
+        ** unfold Relations_1.Transitive.
+          apply node_lt_transitive.
+      * apply Sorted_StronglySorted in Hsorted'; last eauto with *.
+        inversion Hsorted' as [| ??? Hall]; subst.
+        assert (List.In a (a' :: l')) as [|]; subst.
+        { apply elem_of_list_In. rewrite -Hperm. by left. }
+        ** congruence. 
+        ** eapply List.Forall_forall in Hall; eauto.
+        ** unfold Relations_1.Transitive.
+          apply node_lt_transitive.
+  Qed.
+
+  Lemma node_rep_sorted_app (L1 L2: list node_rep) :
+    Sorted node_lt (L1 ++ L2) → Sorted node_lt L1 ∧ Sorted node_lt L2.
+  Proof.
+    induction L1.
+    + rewrite //=; intros; intuition; econstructor.
+    + intros Hs.
+      apply Sorted_StronglySorted in Hs; last first.
+      { unfold Relations_1.Transitive; apply node_lt_transitive. }
+      inversion Hs; subst; eauto.
+      destruct IHL1 as [HL1 HL2].
+      - by apply StronglySorted_Sorted.
+      - split; apply StronglySorted_Sorted.
+        * apply Sorted_StronglySorted in HL1; last first.
+          { unfold Relations_1.Transitive; apply node_lt_transitive. }
+          constructor; first done.
+          apply list.Forall_forall. intros. eapply list.Forall_forall; eauto.
+          apply elem_of_list_In. apply in_or_app. left. apply elem_of_list_In; done. 
+        * apply Sorted_StronglySorted.
+          unfold Relations_1.Transitive; apply node_lt_transitive.
+          done.
+  Qed.
+
+  Lemma forall_node_lt_Zlt (L: list node_rep) (rep: node_rep) :
+    Forall (node_lt rep) L →
+    Forall (Z.lt (node_key rep)) (map node_key L).
+  Proof.
+    induction 1; econstructor; eauto.
+  Qed.
+
+  Lemma node_rep_split_join (L: list node_rep) (head: node_rep) (k: Z):
+    node_key head < k < INT_MAX →
+    ∃ (pred succ: node_rep) (L1 L2: list node_rep),
+      node_key pred < k ≤ node_key succ ∧
+      [head] ++ L ++ [tail] = L1 ++ [pred; succ] ++ L2.
+  Proof.
+    revert head.
+    induction L as [| curr L] => head.
+    - intros (?&?). exists head, tail, nil, nil.
+      split_and!; auto. rewrite /tail/node_key//=; eauto. lia.
+    - intros (?&?).
+      destruct (Z_lt_dec (node_key curr) k).
+      * edestruct IHL as (pred&succ&L1&L2&Hrange&Heq); eauto.
+        destruct Hrange.
+        exists pred, succ, (head :: L1), L2.
+        split_and!;eauto. simpl in *. rewrite Heq. auto.
+      * exists head, curr, nil, (L ++ [tail]).
+        split_and!; eauto; lia.
+  Qed.
+
+  Lemma node_rep_split_sep (L Li Lf L1 Le: list node_rep) 
+    (head curr pred succ: node_rep) (k: Z) :
+    Sorted node_lt ([head] ++ L ++ [tail]) →
+    node_key curr < k < INT_MAX →
+    node_key pred < k ≤ node_key succ  →
+    [head] ++ L = Li ++ [curr] ++ Lf →
+    [curr] ++ Lf ++ [tail] = L1 ++ [pred; succ] ++ Le →
+    ∃ (Lm: list node_rep), 
+      Li ++ [curr] ++ Lm ++ [succ] ++ Le = [head] ++ L ++ [tail].
+  Proof.
+    intros Hsort Hr1 Hr2 Heq1 Heq2.
+    destruct L1 as [| a L1].
+    + exists nil. simpl in *.
+      inversion Heq2. symmetry.
+      rewrite app_comm_cons Heq1 app_ass.
+      subst; auto.
+    + inversion Heq2; subst.
+      exists (L1 ++ [pred]). symmetry. 
+      rewrite -app_ass Heq1 app_ass. f_equal.
+      rewrite app_ass. f_equal.
+      rewrite H1 app_ass //=.
+  Qed.
+
+  Lemma sorted_node_lt_cover_gap (L1 L2: list node_rep) (pred succ: node_rep) (k: Z):
+    Sorted node_lt (L1 ++ [pred; succ] ++ L2) →
+    node_key pred < k ≤ node_key succ →
+    In k (map node_key (L1 ++ [pred; succ] ++ L2)) →
+    node_key succ = k.
+  Proof.
+    induction L1.
+    - rewrite //= => Hsort Hr Hin. inversion Hin as [|[Heq|Hin']]; subst; try lia.
+      exfalso. apply Sorted_StronglySorted in Hsort; last first.
+      { unfold Relations_1.Transitive; apply node_lt_transitive. }
+      apply StronglySorted_inv in Hsort as (Hsort&_).
+      apply StronglySorted_inv in Hsort as (Hsort&hd).
+      assert (node_key succ < k); last by lia.
+      apply forall_node_lt_Zlt in hd.
+      eapply Forall_forall; eauto.
+      by apply elem_of_list_In.
+    - rewrite //=. intros Hsort ? Hin.
+      inversion Hin.
+      * subst.
+        exfalso. apply Sorted_StronglySorted in Hsort; last first.
+        { unfold Relations_1.Transitive; apply node_lt_transitive. }
+        apply StronglySorted_inv in Hsort as (Hsort&Hhd).
+        assert (node_lt a pred); last first.
+        { unfold node_lt in *. lia. }
+        eapply Forall_forall; eauto.
+        apply elem_of_list_In.
+        apply in_app_iff. right. by left.
+      * eapply IHL1; eauto.
+        apply Sorted_inv in Hsort; intuition.
+  Qed.
+
+  Lemma sorted_node_lt_hd_nin (x: node_rep) (L: list node_rep):
+    Sorted node_lt (x :: L) → x ∉ L.
+  Proof.
+    induction L => Hsort.
+    eauto with *.
+    apply not_elem_of_cons; split.
+    * apply Sorted_inv in Hsort as (?&Hhd).
+      inversion Hhd; subst.
+      unfold node_lt in H1.
+      assert (node_key x ≠ node_key a) by lia. congruence.
+    * eapply IHL.
+      apply Sorted_inv in Hsort as (Hsort&Hhd).
+      apply Sorted_inv in Hsort as (?&Hhd').
+      apply Sorted_cons; eauto.
+      inversion Hhd'. subst.
+      ** econstructor. 
+      ** econstructor. inversion Hhd.
+        by eapply node_lt_transitive.
+  Qed.
+
+  Lemma sorted_node_lt_no_dup (L: list node_rep):
+    Sorted node_lt L → NoDup L.
+  Proof.
+    induction L as [|a L] => Hsorted.
+    - econstructor.
+    - specialize (sorted_node_lt_hd_nin a L Hsorted); auto.
+      apply Sorted_inv in Hsorted as (Hsorted&?).
+      econstructor; eauto.
+  Qed.
+
+  Lemma sorted_node_lt_hd (L: list node_rep) (h a: node_rep) :
+    In a (h :: L) →
+    Sorted node_lt (h :: L) →
+    a = h ∨ node_lt h a.
+  Proof.
+    intros Hin Hsort.
+    apply Sorted_StronglySorted in Hsort; last first.
+    { unfold Relations_1.Transitive; apply node_lt_transitive. }
+    apply StronglySorted_inv in Hsort as (?&Hforall).
+    destruct Hin; first by left. right.
+    rewrite List.Forall_forall in Hforall.
+    by eapply Hforall.
+  Qed.
+
+  Lemma sorted_node_key_unique (L: list node_rep) (a b: node_rep):
+    Sorted node_lt L →
+    In a L →
+    In b L →
+    node_key a = node_key b →
+    a = b.
+  Proof.
+    induction L as [|h L] => Hsort Hina Hinb Hkey.
+    + by exfalso.
+    + inversion Hina; subst.
+      - clear IHL.
+        apply sorted_node_lt_hd in Hinb; last auto.
+        destruct Hinb as [?|Hfalse]; first auto. 
+        unfold node_lt in Hfalse; lia.
+      - inversion Hinb; subst.
+        * clear IHL.
+          apply sorted_node_lt_hd in Hina; last auto.
+          destruct Hina as [?|Hfalse]; first auto. 
+          unfold node_lt in Hfalse; lia.
+        * apply Sorted_inv in Hsort; destruct Hsort.
+          apply IHL; auto.
+  Qed.
+  
+End NodeLt.
