lazy_list/spec/new.v
@@ -1,0 +1,63 @@
+From iris.algebra Require Import auth frac_auth gset.
+From iris.heap_lang Require Import proofmode.
+
+From SkipList.lib Require Import lock misc.
+From SkipList.lazy_list Require Import inv node_rep code key_equiv.
+
+
+Local Open Scope Z.
+Module NewSpec (Params: LAZY_LIST_PARAMS).
+  Import Params.
+  Module Invariant := LazyListInv Params.
+  Import Invariant.
+
+  Section Proofs.
+    Context `{!heapGS Σ, !gset_list_unionGS Σ, lockG Σ} (N : namespace).
+
+    Theorem new_spec :
+      {{{ True }}}
+        new #()
+      {{{ Γ v, RET v; 
+        is_lazy_list N v ∅ 1 Γ
+      }}}.
+    Proof.
+      iIntros (Φ) "_ HΦ".
+
+      iMod (own_alloc (● (∅ : gset node_rep) ⋅ ◯ (∅: gset node_rep)))
+        as (γauth) "[Hown_auth Hown_auth_frag]"; 
+        first by apply auth_both_valid.
+      iMod (own_alloc (●F (∅ : gset node_rep) ⋅ ◯F (∅: gset node_rep)))
+        as (γfrac) "[Hown_frac Hown_frac_frag]"; 
+        first by apply auth_both_valid.
+      iMod (own_alloc (GSet (Zlt_range INT_MIN INT_MAX)))
+        as (γtok) "Hown_tok"; first done.
+
+      assert (GSet (Zlt_range INT_MIN INT_MAX) =
+        GSet (Zlt_range INT_MIN INT_MAX) ⋅ GSet (∅)) as ->.
+      { rewrite gset_disj_union; f_equal; set_solver. }
+      iDestruct "Hown_tok" as "(Hown_tok & Hown_emp)".
+
+      wp_lam. wp_alloc t as "Ht". wp_let.
+      iDestruct "Ht" as "(Ht1 & Ht2)".
+      wp_apply (newlock_spec (node_inv t γtok (INT_MIN)) with "[Ht1 Hown_tok]").
+      { iExists tail; iFrame. }
+      iIntros (l) "#Hlock". iDestruct "Hlock" as (γ) "Hlock".
+      set (head := (INT_MIN, Some t, l)).
+      wp_pures; rewrite (fold_rep_to_node head).
+
+      iMod (inv_alloc N ⊤ (lazy_list_inv head γauth γfrac γtok) 
+        with "[Ht2 Hlock Hown_auth Hown_frac Hown_emp]") as "#Hinv".
+      + iNext. iExists ∅, ∅, nil. iFrame.
+        iSplit; first done. iSplit. 
+        assert (node_lt head tail); last (simpl; auto).
+        { rewrite /node_lt/node_key//=; apply HMIN_MAX. }
+        iSplit; first by unfold key_equiv.
+        iExists t, γ. by iFrame "# ∗".
+      + iModIntro; iApply ("HΦ" $! (mk_lazy_gname γauth γfrac γtok)).
+        iExists head, ∅.
+        iSplit; first by unfold key_equiv.
+        by (repeat iSplit).
+    Qed.
+
+  End Proofs.
+End NewSpec.
